src/Layers/AbstractLayers/FileDisk/FileDiskLayer.v
@@ -27,7 +27,8 @@ Section FileDisk.
   | ChangeOwner : Inum -> user -> file_disk_prog (option unit)
   | Create : user -> file_disk_prog (option addr)
   | Delete : Inum -> file_disk_prog (option unit)
-  | Recover : file_disk_prog unit.
+  | Recover : file_disk_prog unit
+  | Init : file_disk_prog unit.
   
   Inductive exec' :
     forall T, user -> token' ->  state' -> file_disk_prog T -> @Result state' T -> Prop :=
@@ -157,6 +158,10 @@ Section FileDisk.
   | ExecRecover : 
       forall d u,
         exec' u Cont d Recover (Finished d tt)
+  
+  | ExecInit : 
+        forall d u,
+          exec' u Cont d Init (Finished empty_mem tt)
 
   | ExecCrashBefore :
       forall u d T (p: file_disk_prog T),
