bench/compile-and-run.sh
@@ -1,20 +1,35 @@
-cd ../src/Extraction/
-./compile.sh
-cd ../../bench
-mv ../src/Extraction/extracted/ConFs ./fs/ConFs
-mv ../src/Extraction/extracted/mkfs ./fs/ConMkfs
+#cd ../src/Extraction/
+#./compile.sh
+#cd ../../bench
+#mv ../src/Extraction/extracted/ConFs ./fs/ConFs
+#mv ../src/Extraction/extracted/mkfs ./fs/ConMkfs
 
-cd ../../fscq/fscq15/src/
+#cd ../../fscq/fscq15/src/
 #make
-cd ../../../ConFrm/bench
-mv ../../fscq/fscq15/src/fuse ./fs/CfscqFs
-mv ../../fscq/fscq15/src/mkfs ./fs/CfscqMkfs
+#cd ../../../ConFrm/bench
+#mv ../../fscq/fscq15/src/fuse ./fs/CfscqFs
+#mv ../../fscq/fscq15/src/mkfs ./fs/CfscqMkfs
+
+if [ $# -ne 2 ]; then
+  echo "$0 dev num-of-times"
+  exit 1
+fi
 
 ./compile-sources.sh
 sudo rm -rf results
-sudo ./run-confs.sh $2 $1
-sudo ./run-cfscq.sh $2 $1
+#sudo ./run-confs.sh $2 $1
+#sleep 1m
+#sudo ./run-confssync.sh $2 $1
+#sleep 1m
+#sudo ./run-cfscq.sh $2 $1
+#sleep 1m
 sudo ./run-sfscq.sh $2 $1
+sleep 1m
+sudo ./run-dfscq.sh $2 $1
+sleep 1m
 sudo ./run-ext4.sh $2 $1
+sleep 1m
+sudo ./run-ext4journal.sh $2 $1
+sleep 1m
 
 ./get-stats.sh
