bench/run-sfscq.sh
@@ -12,11 +12,11 @@ mkdir results/Sfscq
 
 echo "=== Running Sfscq Tests ==="
 
-echo "== smallfile =="
-./run_script.sh Sfscq smallfile $DEV $ITER > results/Sfscq/smallfile
+#echo "== smallfile =="
+#./run_script.sh Sfscq smallfile $DEV $ITER > results/Sfscq/smallfile
 echo "== largefile =="
 ./run_script.sh Sfscq largefile $DEV $ITER > results/Sfscq/largefile
-echo "== createdelete =="
-./run_script.sh Sfscq createdelete $DEV $ITER > results/Sfscq/createdelete
-echo "== rename =="
-./run_script.sh Sfscq rename $DEV $ITER > results/Sfscq/rename
+#echo "== createdelete =="
+#./run_script.sh Sfscq createdelete $DEV $ITER > results/Sfscq/createdelete
+#echo "== rename =="
+#./run_script.sh Sfscq rename $DEV $ITER > results/Sfscq/rename
